test-suite/erasure_live_test.v
@@ -317,9 +317,10 @@ End HetList.
 Require Import Coq.Arith.Compare_dec.
 Require Import Coq.Arith.PeanoNat.
 Require Import Coq.Arith.Peano_dec.
-Require Import Arith.
+Require Import Arith Wf.
 Program Fixpoint provedCopy (n:nat) {wf lt n} : nat :=
   match n with 0 => 0 | S k => S (provedCopy k) end.
+Next Obligation. eapply measure_wf, lt_wf. Qed. 
 Print Assumptions provedCopy.
 MetaCoq Quote Recursively Definition pCopy := provedCopy. (* program *)
 
@@ -331,7 +332,7 @@ MetaCoq Quote Recursively Definition cbv_provedCopyx :=
 Definition ans_provedCopyx :=
   Eval lazy in (test cbv_provedCopyx).
 MetaCoq Quote Recursively Definition p_provedCopyx := provedCopyx. (* program *)
-Time Definition P_provedCopyx := Eval vm_compute in (test_fast cbv_provedCopyx).
+Time Definition P_provedCopyx := Eval lazy in (test_fast cbv_provedCopyx).
 (* We don't run this one every time as it is really expensive *)
 (*Time Definition P_provedCopyxvm := Eval vm_compute in (test p_provedCopyx).*)
 
