test-suite/self_erasure.v
@@ -1,7 +1,7 @@
 From MetaCoq.Erasure Require Import Loader Erasure.
 From MetaCoq.SafeChecker Require Import PCUICSafeChecker.
 Set MetaCoq Timing.
-(* 32sec *)
-MetaCoq Erase @erase_and_print_template_program.
-(* 40sec *)
+(* 1sec *)
+MetaCoq Fast Erase @erase_and_print_template_program.
+(* 4sec *)
 Time MetaCoq Erase @typecheck_program.
